src/tls/TLS.Handshake.Outline.fst
@@ -1,0 +1,184 @@
+module TLS.Handshake.Outline
+
+open FStar.Error
+open FStar.Bytes // still used for cookies, tickets, signatures...
+
+open Mem
+open TLSError
+open TLSInfo
+open TLSConstants
+
+module B = LowStar.Buffer
+module HS = FStar.HyperStack
+module HST = FStar.HyperStack.ST
+
+module HSM = HandshakeMessages
+module LP = LowParse.Low.Base
+module Transcript = HSL.Transcript
+
+module Range = Range
+
+include TLS.Handshake.Receive.Wrapper
+include TLS.Handshake.Machine
+
+/// Outlining our integration test (code adapted from TLS.Handshake).
+/// See also https://github.com/project-everest/mitls-fstar/issues/231
+/// and
+/// https://github.com/project-everest/mitls-fstar/blob/afromher_dev/src/tls/Test.TLS.Send.fst
+
+(* ----------------------- Incoming ----------------------- *)
+
+
+(* OLD:
+let recv_ensures (#region:rgn) (cfg:client_config) (cs:client_state region cfg) (h0:HS.mem) (result:incoming) (h1:HS.mem) =
+    let w0 = iT s Writer h0 in
+    let w1 = iT s Writer h1 in
+    let r0 = iT s Reader h0 in
+    let r1 = iT s Reader h1 in
+    hs_inv s h1 /\
+    mods s h0 h1 /\
+    w1 == w0 /\
+    r1 == (if in_next_keys result then r0 + 1 else r0) /\
+    (b2t (in_complete result) ==> r1 >= 0 /\ r1 = w1 /\ iT s Reader h1 >= 0 (*/\ completed (eT s Reader h1)*) )
+*)
+
+val receive_fragment:
+  // mutable client state
+  #region:rgn -> hs: TLS.Handshake.Machine.t region ->
+  // high-level calling convention for the incoming fragment
+  #i:TLSInfo.id -> rg:Range.frange i -> f:Range.rbytes rg ->
+  ST incoming
+  (requires fun h0 ->
+    // TODO statically exclude C_init
+    True)
+  (ensures fun h0 r h1 -> True)
+
+let buffer_received_fragment ms #i rg f = ms
+
+// TODO ms has a dependent type
+
+// TODO copy f's contents into !hs.receiving.rcv_b between rcv_to and
+// the end of the slice, probably returning indexes too, possibly
+// reallocating a bigger buffer if the current one is too small
+// (later?)
+
+
+// the actual transitions; we should experiment with some precise pre/post
+assume val client_HelloRetryRequest: #region:rgn -> hs: t region -> HSM.hrr -> St incoming
+assume val client_ServerHello:       #region:rgn -> hs: t region -> HSM.sh -> St incoming
+assume val client_ServerHelloDone:   #region:rgn -> hs: t region -> HSM.sh -> St incoming
+assume val client_ServerFinished13:  #region:rgn -> hs: t region ->
+  full_offer ->
+  sh: serverHello ->
+  ee: HSM.encryptedExtensions ->
+  ocr: option HSM.certificateRequest13 ->
+  oc: option HSM.certificate13 ->
+  ocv: option HSM.certificateVerify13 ->
+  svd: bytes ->
+  digestCert: option Hashing.anyTag ->
+  digestCertVerify: Hashing.anyTag ->
+  digestServerFinished: Hashing.anyTag ->
+  St incoming
+
+open TLS.Handshake.Receive.Wrapper
+
+#set-options "--admit_smt_queries true"
+let rec receive_fragment #region hs #i rg f =
+  let open HandshakeMessages in
+  let recv_again r =
+    match r with
+    // only case where the next incoming flight may already have been buffered.
+    | InAck false false -> receive_fragment hs #i (0,0) empty_bytes
+    | r -> r  in
+  // trace "recv_fragment";
+  let h0 = HST.get() in
+
+  match !(cst hs) with
+  | C_init _ ->
+    InError (fatalAlert Unexpected_message, "Client hasn't sent hello yet (to be statically excluded)")
+
+  | C_wait_ServerHello offer0 ms0 ks0 -> (
+    let ms1 = buffer_received_fragment ms0 #i rg f in
+    let cslice = admit() (* from ms1.receiving.rcv_b *) in
+    // TODO: adjust parameters; refactor HSL.Receive to take ms1.receiving as parameter?
+    match TLS.Handshake.Receive.receive_c_wait_ServerHello // to be refined to advance the rcv_state
+      ms1.receiving.hsl_rcv_st
+      cslice
+      ms1.receiving.rcv_from
+      ms1.receiving.rcv_to
+    with
+    | Error z -> InError z
+    | Correct None -> InAck false false // nothing happened
+    | Correct (Some sh_msg) -> (
+      let sh = admit() in
+      if HSM.is_hrr sh then
+        // TODO adjust digest, here or in the transition call
+        client_HelloRetryRequest hs (HSM.get_hrr sh)
+      else
+        // TODO extend digest[..sh]
+        // transitioning to C12_wait_ServerHelloDone or C13_wait_Finished1;
+        let r = client_ServerHello hs (HSM.get_sh sh) in
+        // TODO check that ms1.receiving is set for processing the next flight
+        recv_again r ))
+
+  | C12_wait_ServerHelloDone ch sh ms0 ks -> (
+    let ms1 = buffer_received_fragment ms0 #i rg f in
+    let cslice = admit() (* from ms1.receiving.rcv_b *) in
+    match TLS.Handshake.Receive.receive_c12_wait_ServerHelloDone
+      ms1.receiving.hsl_rcv_st
+      cslice
+      ms1.receiving.rcv_from
+      ms1.receiving.rcv_to
+    with
+    | Error z -> InError z
+    | Correct None -> InAck false false // nothing happened
+    | Correct (Some x) ->
+      // TODO extend digest[..ServerHelloDone]
+      // let c, ske, ocr = admit() in
+      // client_ServerHelloDone hs c ske None
+      admit()
+      )
+
+  | C13_wait_Finished1 offer sh ms0 ks -> (
+    let ms1 = buffer_received_fragment ms0 #i rg f in
+    let cslice = admit() (* from ms1.receiving.rcv_b *) in
+    match TLS.Handshake.Receive.receive_c13_wait_Finished1
+      ms1.receiving.hsl_rcv_st
+      cslice
+      ms1.receiving.rcv_from
+      ms1.receiving.rcv_to
+    with
+    | Error z -> InError z
+    | Correct None -> InAck false false // nothing happened
+    | Correct (Some x) ->
+      // covering 3 cases (see old code for details)
+      // we need to extract these high-level values from the flight:
+      let ee, ocr, oc, ocv, fin1, otag0, tag1, tag_fin1 = admit() in
+      client_ServerFinished13 hs offer sh ee ocr oc ocv fin1 otag0 tag1 tag_fin1
+      )
+(*
+  | C13_Complete _ _ _ _ _ _ _ ms0 _ ->
+    let ms1 = buffer_received_fragment ms0 #i rg f in
+    // TODO two sub-states: waiting for fin2 or for the post-handshake ticket.
+    match HSL.Receive.receive_c_wait_ServerHello 12_wait_ServerHelloDone st b f_begin f_end with
+    | Error z -> InError z
+    | Correct None -> InAck false false // nothing happened
+    | Correct (Some x) ->
+
+  , [Msg13 (M13_new_session_ticket st13)], [_] ->
+      client_NewSessionTicket_13 hs st13
+
+  // 1.2 full: wrap these two into a single received flight with optional [cr]
+    | C_wait_Finished2 digestClientFinished, [Msg12 (M12_finished f)], [digestServerFinished] ->
+      client_ServerFinished hs f digestClientFinished
+
+    | C_wait_NST resume, [Msg12 (M12_new_session_ticket st)], [digestNewSessionTicket] ->
+      client_NewSessionTicket_12 hs resume digestNewSessionTicket st
+
+    // 1.2 resumption
+    | C_wait_R_Finished1 digestNewSessionTicket, [Msg12 (M12_finished f)], [digestServerFinished] ->
+      client_R_ServerFinished hs f digestNewSessionTicket digestServerFinished
+*)
+
+  | _ ->
+    InError (fatalAlert Unexpected_message, "TBC")
